AP/Util/Data/Set.lean
@@ -1,0 +1,202 @@
+import AP.Util.Data.Map
+
+universe u v w
+
+structure Set' (α : Type u)
+[hh₁ : LinearOrder α] [hh₂ : Hashable α] : Type (max u v) where
+  inner : Std.ExtDHashMap α (λ _ => Unit)
+
+variable {α : Type u} {β : Type v} {γ : Type w}
+variable [ha₁ : LinearOrder α] [ha₂ : Hashable α]
+variable [hb₁ : LinearOrder β] [hb₂ : Hashable β]
+variable [hc₁ : LinearOrder γ] [hc₂ : Hashable γ]
+variable {s : Set' α}
+
+namespace Set'
+
+open Std.DHashMap
+
+def empty : Set' α := ⟨∅⟩
+
+instance : EmptyCollection (Set' α) := ⟨empty⟩
+
+theorem empty_def : (∅ : Set' α) = ⟨∅⟩ := rfl
+
+def insertP (x : α) (s : Set' α) : Set' α :=
+  ⟨insert ⟨x, ()⟩ s.inner⟩
+
+instance : Insert α (Set' α) := ⟨insertP⟩
+
+theorem insert_def {x : α} {s : Set' α} :
+insert x s = ⟨insert ⟨x, ()⟩ s.inner⟩ := rfl
+
+@[simp]
+protected def insert (s : Set' α) (i : α) : Set' α :=
+  ⟨s.inner.insert i ()⟩
+
+def ofList (xs : List α) : Set' α :=
+  ⟨.ofList # xs.map (⟨·, ()⟩)⟩
+
+def mem (s : Set' α) (i : α) : Prop :=
+  i ∈ s.inner
+
+instance : Membership α (Set' α) := ⟨mem⟩
+
+theorem mem_def {i} : i ∈ s ↔ i ∈ s.inner := by rfl
+
+instance {i} : Decidable (s.mem i) := by
+  unfold mem; infer_instance
+
+instance {i} : Decidable (i ∈ s) := by
+  change Decidable # s.mem i; infer_instance
+
+def toList (s : Set' α) : List α :=
+  s.inner.lift (·.toSortedKeys) # by
+    intro s₁ s₂ h; dsimp; unfold toSortedKeys; congr 1; simpa
+
+@[simp]
+theorem ofList_nil : ofList (α := α) [] = ∅ := rfl
+
+@[simp]
+theorem ofList_snoc {xs} {x : α} :
+ofList (xs ++ [x]) = (ofList xs).insertP x := by
+  unfold insertP ofList; simp
+
+@[simp]
+theorem toList_empty : (∅ : Set' α).toList = [] := by
+  change List.map _ _ = _; simp [toSortedList]
+
+@[simp]
+theorem mem_insertP {x : α} {i} :
+i ∈ s.insertP x ↔ i = x ∨ i ∈ s :=
+  Std.ExtDHashMap.mem_insert'
+
+@[simp]
+theorem mem_insert' {i j} :
+j ∈ s.insert i ↔ j = i ∨ j ∈ s := by
+  simp [mem_def]; tauto
+
+@[simp]
+theorem mem_insert {x i} :
+i ∈ Insert.insert x s ↔ i = x ∨ i ∈ s :=
+  mem_insert'
+
+@[simp]
+theorem mem_ofList {xs : List α} {i} :
+i ∈ ofList xs ↔ i ∈ xs := by
+  simp [ofList, mem_def]
+
+theorem eq_empty_iff : s = ∅ ↔ ∀ i, i ∉ s := by
+  rcases s with ⟨mp⟩; simp [empty_def]
+  exact Std.ExtDHashMap.eq_empty_iff
+
+@[simp]
+theorem not_mem_empty' {i} : ¬(∅ : Set' α).mem i :=
+  Std.ExtDHashMap.not_mem_empty
+
+@[simp]
+theorem not_mem_empty {i} : i ∉ (∅ : Set' α) :=
+  not_mem_empty'
+
+theorem ext_iff' {s₁ s₂ : Set' α} :
+s₁ = s₂ ↔ s₁.inner.1.out ~m s₂.inner.1.out := by
+  rcases s₁ with ⟨s₁⟩; rcases s₂ with ⟨s₂⟩; simp
+  exact Std.ExtDHashMap.ext_iff'
+
+theorem ext' {s₁ s₂ : Set' α}
+(h : s₁.inner.1.out ~m s₂.inner.1.out) : s₁ = s₂ := by
+  rwa [ext_iff']
+
+theorem ext_iff {s₁ s₂ : Set' α} : s₁ = s₂ ↔ ∀ i, i ∈ s₁ ↔ i ∈ s₂ := by
+  rcases s₁ with ⟨s₁⟩; rcases s₂ with ⟨s₂⟩
+  simp [mem_def, Std.ExtDHashMap.ext_iff, Option.eq_iff_of_subsingleton]
+
+@[ext]
+theorem ext {s₁ s₂ : Set' α} (h : ∀ i, i ∈ s₁ ↔ i ∈ s₂) : s₁ = s₂ := by
+  rwa [ext_iff]
+
+theorem get?_eq_ite_of_unit {m : Map α Unit} {i} :
+m.get? i = if i ∈ m then some () else none :=
+  Std.ExtDHashMap.get?_eq_ite_of_unit
+
+theorem ofList_eq_ofList_iff {xs ys : List α}
+(hx : xs.Nodup) (hy : ys.Nodup) :
+ofList xs = ofList ys ↔ xs.Perm ys := by
+  simp [ofList]
+  rw [Std.ExtDHashMap.ofList_eq_ofList_iff]
+  any_goals simpa
+  rw [List.map_perm_map_iff]
+  intro x y h; simp at h; exact h
+
+def univ [ha : Fintype α] : Set' α :=
+  ⟨Std.ExtDHashMap.range # λ _ => ()⟩
+  
+@[simp]
+theorem mem_univ [ha : Fintype α] {i : α} : i ∈ univ :=
+  Std.ExtDHashMap.mem_range
+
+@[simp]
+theorem nonempty_insert {x} : Insert.insert x s ≠ ∅ := by
+  simp [ext_iff', ←equiv_def]
+  rcases s with ⟨s⟩
+  rw [insert_def]
+  simp
+  have h₁ := @Std.ExtDHashMap.nonempty_insert α (λ _ => Unit) _ _
+    s ⟨x, ()⟩
+  simp at h₁
+  rwa [Std.ExtDHashMap.inner_eq_iff_eq]
+
+@[simp]
+theorem nodup_toList : s.toList.Nodup := by
+  rcases s with ⟨⟨s⟩⟩; unfold toList Std.ExtDHashMap.lift
+  rw [Quotient.lift_eq]
+  simp
+
+@[simp]
+theorem sorted_toList : s.toList.Sorted (· ≤ ·) := by
+  rcases s with ⟨⟨s⟩⟩; unfold toList Std.ExtDHashMap.lift
+  apply s.ind; simp
+
+@[simp]
+theorem mem_toList {x} : x ∈ s.toList ↔ x ∈ s := by
+  rcases s with ⟨⟨s⟩⟩; unfold toList
+  apply s.ind; clear s; intro s
+  unfold toSortedKeys Std.ExtDHashMap.lift
+  change _ ↔ x ∈ s
+  simp [Option.eq_iff_of_subsingleton]
+
+@[simp]
+theorem toList_eq_toList {s₁ s₂ : Set' α} :
+s₁.toList = s₂.toList ↔ s₁ = s₂ := by
+  rcases s₁ with ⟨⟨s₁⟩⟩; rcases s₂ with ⟨⟨s₂⟩⟩
+  simp [toList, Quotient.lift_eq]
+  exact Quotient.out_equiv_out (x := s₁)
+
+@[simp]
+theorem toList_eq_nil_iff : s.toList = [] ↔ s = ∅ := by
+  rcases s with ⟨⟨s⟩⟩; unfold toList
+  apply s.ind; clear s; intro s
+  simp [empty_def]
+  unfold Std.ExtDHashMap.lift
+  simp
+  change _ ↔ _ = Std.ExtDHashMap.mk' _
+  simp
+  change _ ↔ _ ~m _
+  simp
+
+@[simp]
+def toDMap (s : Set' α) : DMap α (λ _ => Unit) :=
+  ⟨s.inner⟩
+
+@[simp]
+def toMap (s : Set' α) : Map α Unit :=
+  ⟨s.inner⟩
+
+instance : DecidableEq (Set' α) :=
+  λ s₁ s₂ => match h : decide # s₁.inner = s₂.inner with
+  | true => isTrue # by
+    rcases s₁ with ⟨s₁⟩; rcases s₂ with ⟨s₂⟩
+    simp at h; simpa
+  | false => isFalse # by
+    rcases s₁ with ⟨s₁⟩; rcases s₂ with ⟨s₂⟩
+    simp at h; simpa
